\documentclass{article}

\usepackage{amsmath}
\usepackage{amssymb}

\usepackage{fancyhdr}
\pagestyle{fancy}
\fancyhf{}
\lhead{CS421 (02) HW1A}
\rhead{Boris Nikulin \thepage}

\begin{document}

\begin{enumerate}
	\item[Inter2.]
		Prefixes of \texttt{abc} are $\{\lambda, a, ab, abc\}$.

	\item[Problem 2.]
		Prove $$\sum_{k=0}^n 2^k = 2^{n+1} - 1, n \geq 0$$

		Basis $P(0)$ when $n = 0$
		$$\sum_{k=0}^0 2^k = 2^0 = 1 = 2^1 - 1 = 2^{0+1} â€“ 1$$
		is true.

		Assume $P(i)$ is true, $A_L = A_R$ when $n = i$
		$$A_L = \sum_{k=0}^i 2^k = 2^{i+1} - 1 = A_R$$

		Inductive step $P(i)$ to $P(i + 1)$
		\begin{align*}
			\sum_{k=0}^{i+1} 2^k &= 2^{i+2} - 1 \\
				&= A_L + 2^{i+1} \\
				&= A_R + 2^{i+1} = 2^1 \cdot 2^{i+1} \\
				&= 2^{i+2} - 1
		\end{align*}
		$$\therefore \sum_{k=0}^n 2^k = 2^{n+1} - 1, n \geq 0$$
\end{enumerate}

\end{document}
